
\chapter{Appendix B}
\label{app:app02}

\initial{H}ere we present the analytic solution in one dimension used in our model. We first solve the general solution. In our model we first studied the case with infinite boundary conditions, the solution for this particular case is provided, the proceeding solutions of our case studies, that is with boundary conditions and the effect of grain boundaries in the bulk are also given.

\section{One dimension}
From 
\begin{equation}\label{eqtn5}
   D\triangledown^2n(y) - \frac{n(y)}{\tau} -G_0(y) = 0
  \end{equation}
 Homogeneous solution \\
 let 
\begin{equation}\label{eqtn6}
  n(y)= \exp(\lambda y) 
   \end{equation}
  \begin{equation}\label{eqtn7}
  n^{''}(y) = \lambda^2 \exp(\lambda y)
 \end{equation}
 \begin{equation}\label{eqtn8}
\lambda^2 \exp(\lambda y) -\frac{n(y)}{\tau D}\exp(\lambda y)  = 0 \Rightarrow \lambda = \pm \frac{1}{\sqrt{\tau D}} = \frac{1}{L_n}. 
\end{equation}
\begin{equation}\label{eqtn11}
n(y) = C_1\exp\left(\frac{y}{L_n}\right) + C_2\exp \left(\frac{-y}{L_n}\right)
\end{equation}
particular solution.
\begin{equation*}
n(y) = A\frac{G_0}{D} 
\end{equation*}
\begin{equation*}
n(y) = -\frac{AG_0}{\tau D^2} + \frac{G_0}{D} = 0 
\end{equation*}
\begin{equation*}
A = \tau D
\end{equation*}
\begin{equation}
\label{eqtn:eq09}
n(y) = L_n^2\frac{G_0}{D} 
\end{equation}
Therefore the general solution for equation \ref{eqtn5} is;
\begin{equation}\label{eqtn10}
n(y) = C_1\exp \left(\frac{y}{L_n}\right) + C_2\exp\left(\frac{-y}{L_n}\right) +  L_n^2\frac{G_0}{D} 
\end{equation}

\subsection{With no surface recombination}

In our model with infinity boundary condition, we have three expression, in the three different regions.
\begin{equation}\label{eqtn12}
n(y) = A_1\exp \left(\frac{y}{L_n}\right)
\end{equation}
\begin{equation} \label{eqtn13}
n(y) = B_1\exp \left(\frac{y}{L_n}\right) + B_2\exp \left(\frac{-y}{L_n}\right) +   L_n^2\frac{G_0}{D} 
\end{equation}
\begin{equation} \label{eqtn14}
n(y) = C_2\exp \left(\frac{-y}{L_n}\right)
\end{equation}

Since these equations must be continuous; we can include the continuity conditions in order to solve for the coefficients;
\begin{equation} \label{eqtn15}
 A_1\exp \left(\frac{y_1}{L_n}\right) =  B_1\exp \left(\frac{y_1}{L_n}\right) + B_2\exp \left(\frac{-y_1}{L_n}\right) + g_0 \longleftrightarrow g_0 =  L_n^2\frac{G_0}{D} 
\end{equation}
\begin{equation} \label{eqtn16}
 A_1\exp \left(\frac{y_1}{L_n}\right) =  B_1\exp \left(\frac{y_1}{L_n}\right) - B_2\exp \left(\frac{-y_1}{L_n}\right) + 0
\end{equation}
\begin{equation*}
 2B_2\exp \left(\frac{-y_1}{L_n}\right) = -g_0 
 \end{equation*}
\begin{equation}
 \label{eqtn17}
 B_2 = -\frac{g_0}{2}\exp \left(\frac{-y_1}{L_n}\right) 
\end{equation}
\begin{equation}
\label{eqtn:eq02r}
A_1 = B_1 -B_2\exp \left(\frac{-2y_1}{L_n}\right)
\end{equation}

\begin{equation} \label{eqtn18}
 C_2\exp \left(\frac{y_2}{L_n}\right) =  B_1\exp \left(\frac{y_2}{L_n}\right) + B_2\exp \left(\frac{-y_2}{L_n}\right) + g_0
\end{equation}
\begin{equation} \label{eqtn19}
 C_2\exp \left(\frac{y_2}{L_n}\right) =  B_1\exp \left(\frac{y_2}{L_n}\right) - B_2\exp \left(\frac{-y_2}{L_n}\right) + 0
\end{equation}
\begin{equation*}
 2B_1\exp \left(\frac{-y_2}{L_n}\right) = -g_0 
\end{equation*} 
\begin{equation}
 \label{eqtn20}
B_1 = -\frac{g_0}{2}\exp \left(\frac{-y_2}{L_n}\right) 
\end{equation}
\begin{equation}
\label{eqn:eq03r}
 C_2 = B_2 -B_1\exp \left(\frac{-2y_2}{L_n}\right)
\end{equation}

\subsection{Applying surface recombination}\label{app:surface}

Solution of equation \ref{eqtn5} with non infinity Boundaries. i.e if we now take into consideration the surface recombination velocity. 
\begin{equation} \label{eqtn22}
 n(y) = A_1\exp \left(\frac{y_2}{L_n}\right) + A_2\exp \left(\frac{-y_2}{L_n}\right)
\end{equation}
\begin{equation} \label{eqtn23}
 n(y) =  B_1\exp \left(\frac{y_2}{L_n}\right) + B_2\exp \left(\frac{-y_2}{L_n}\right) + g_0.
\end{equation}
\begin{equation} \label{eqtn24}
 n(y) = C_1\exp \left(\frac{y_2}{L_n}\right) + C_2\exp \left(\frac{-y_2}{L_n}\right) 
\end{equation} 
at $y_0$
\begin{equation}\label{eqtnb1}
\frac{\partial n}{\partial y} = -\frac{S}{D}n(y_0) = \frac{A_1}{L_n}\exp \left(\frac{y_0}{L_n}\right)  - \frac{A_2}{L_n}\exp \left(\frac{-y_0}{L_n}\right)=-\frac{S}{D}\left(A_1\exp \left(\frac{y_0}{L_n}\right) + A_2\exp \left(\frac{-y_0}{L_n}\right)\right)
\end{equation}
were S is the surface recombination  velocity.
\begin{equation}\label{eqtnb2}
A_2 = A_1\exp \left(\frac{2y_0}{L_n}\right)\frac{\left(1-\frac{SL_n}{D}\right)}{\left(1+\frac{SL_n}{D}\right)} = \frac{-w}{x} A_1 \exp \left(\frac{2y_O}{L_n}\right)
\end{equation}
with $x =\left( \frac{SL_n}{D}+1\right)$ and $w  =\left(\frac{SL_n}{D}-1\right)$ 
at $y_1$
\begin{equation} \label{eqtnb3}
2A_2\exp \left(\frac{-y_1}{L_n}\right) = 2B_2\exp \left(\frac{-y_1}{L_n}\right) + g_0
\end{equation}
\begin{equation}\label{eqtnb4}
B_2 = A_2 - \frac{g_0}{2}\exp \left(\frac{y_1}{L_n}\right)
\end{equation}

Considering the continuity condition around $y_1$, taking the derivatives in A and B, we have,
\begin{equation} \label{eqtnb5}
 A_1\exp \left(\frac{y_1}{L_n}\right) - A_2\exp \left(\frac{-y_1}{L_n}\right) =  B_1\exp \left(\frac{y_1}{L_n}\right) - B_2\exp \left(\frac{-y_1}{L_n}\right)
\end{equation}
\begin{equation*} \label{eqtnb6}
 A_1 =  B_1 - B_2\exp \left(\frac{-2y_1}{L_n}\right)  + A_2\exp \left(\frac{-2y_1}{L_n}\right)
\end{equation*}
Using equations \ref{eqtnb2} and \ref{eqtnb4} we get 
\begin{equation}\label{eqtnb7}
A_1 = B_1 + \frac{g_0}{2}\exp \left(\frac{-y_1}{L_n}\right)
\end{equation}
at $y_3$
\begin{equation}\label{eqtnb8}
\frac{\partial n}{\partial y} = \frac{S}{D}n(y_3) = \frac{C_1}{L_n}\exp \left(\frac{y_3}{L_n}\right)  - \frac{C_2}{L_n}\exp \left(\frac{-y_3}{L_n}\right)= \frac{S}{D}\left(C_1\exp \left(\frac{y_3}{L_n}\right) + C_2\exp \left(\frac{-y_3}{L_n}\right)\right)
\end{equation}
\begin{equation}\label{eqtnb9}
C_1 = -\frac{w}{x}C_2\exp \left(\frac{-2y_3}{L_n}\right)
\end{equation}
at $y_2$
\begin{equation*} \label{eqtnb10}
2B_1\exp \left(\frac{y_2}{L_n}\right) + g_0 = 2C_1\exp \left(\frac{y_2}{L_n}\right)
\end{equation*}
\begin{equation} \label{eqtnb11}
B_1 = C_1 - \frac{g_0}{2}\exp \left(\frac{-y_2}{L_n}\right)
\end{equation}
Considering the continuity condition around $y_2$, taking the derivatives in B and C, we have,
\begin{equation} \label{eqtnb12}
 C_1\exp \left(\frac{y_2}{L_n}\right) - C_2\exp \left(\frac{-y_2}{L_n}\right) =  B_1\exp \left(\frac{y_2}{L_n}\right) - B_2\exp \left(\frac{-y_2}{L_n}\right)
\end{equation}
and using equations \ref{eqtnb2} to \ref{eqtnb11} we can find; 
\begin{equation}\label{eqtnb13}
C_2 = \frac{g_0}{2}\frac{wp}{x}\left(\exp \left(\frac{2y_0}{L_n} - \frac{y_2}{L_n}\right)-\exp \left(\frac{2y_0}{L_n} -\frac{y_1}{L_n}\right)\right) + \frac{g_0}{2p}\left(\exp \left(\frac{y_2}{L_n} - \frac{y_1}{L_n}\right)\right)
\end{equation}
with $p = 1 - \frac{w^2}{x^2}\exp \left(\frac{-2y_3}{L_n} +\frac{2y_0}{L_n}\right)$

\subsection{Creating grain boundaries}

Here for regions were modeled (reference) and the solutions are 
\begin{equation} \label{eqtng1}
 n(y) = A_1\exp \left(\frac{y}{L_1}\right)
\end{equation}
\begin{equation} \label{eqtng2}
 n(y) =  B_1\exp \left(\frac{y}{L_1}\right) + B_2\exp \left(\frac{-y}{L_1}\right) + g_0.
\end{equation}
\begin{equation} \label{eqtng3}
 n(y) = C_1\exp \left(\frac{y}{L_2}\right) + C_2\exp \left(\frac{-y}{L_2}\right) 
\end{equation} 
\begin{equation} \label{eqtng4}
 n(y) = D_1\exp \left(\frac{-y}{L_1}\right)
\end{equation}

at $y_1$
\begin{equation} \label{eqtng5}
 A_1\exp \left(\frac{y_1}{L_1}\right) =  B_1\exp \left(\frac{y_1}{L_1}\right) + B_2\exp \left(\frac{-y_1}{L_1}\right) + g_0
\end{equation}
\begin{equation} \label{eqtng6}
 A_1\exp \left(\frac{y_1}{L_1}\right) =  B_1\exp \left(\frac{y_1}{L_1}\right) - B_2\exp \left(\frac{-y_1}{L_1}\right) + 0
\end{equation}
\begin{equation}\label{eqtng7}
A_1 = B_1 - B_2\exp \left( \frac{-2y_1}{L_1}\right)
\end{equation}
\begin{equation}
B_2 = -\frac{g_0}{2}\exp \left( \frac{y_1}{L_1}\right)
\end{equation}
at $y_2$
\begin{equation} \label{eqtng8}
B_1\exp \left(\frac{y_1}{L_1}\right) + B_2\exp \left(\frac{-y_1}{L_1}\right) + g_0 = C_1\exp \left(\frac{y_2}{L_2}\right) + C_2\exp \left(\frac{-y_2}{L_2}\right)
\end{equation}
\begin{equation} \label{eqtng9}
\frac{B_1}{L_1}\exp \left(\frac{y_1}{L_1}\right) - \frac{B_2}{L_1}\exp \left(\frac{-y_1}{L_1}\right) + 0 = \frac{C_1}{L_2}\exp \left(\frac{y_2}{L_2}\right) - \frac{C_2}{L_2}\exp \left(\frac{-y_2}{L_2}\right)
\end{equation}
from equations \ref{eqtng8} and \ref{eqtng9} we get;
\begin{equation} \label{eqtng10}
B_1 = C_1\exp \left(\frac{y_2}{L_2} -\frac{y_2}{L_1}\right) + C_2\exp \left(\frac{-y_2}{L_1} -\frac{y_2}{L_1}\right) - B_2\exp \left(\frac{-2y_2}{L_1}\right) -g_0\exp \left(\frac{-y2}{L_1}\right)
\end{equation}
at $y_3$
\begin{equation} \label{eqtng11}
C_1\exp \left(\frac{y_3}{L_2}\right) + C_2\exp \left(\frac{-y_3}{L_2}\right)  =  D_2\exp \left(\frac{-y_3}{L_1}\right)
\end{equation}
\begin{equation} \label{eqtng12}
\frac{C_1}{L_2}\exp \left(\frac{y_3}{L_2}\right) - \frac{C_2}{L_2}\exp \left(\frac{-y_3}{L_2}\right)= \frac{D_2}{L_1}\exp \left(\frac{-y_3}{L_1}\right) 
\end{equation}
which gives;
\begin{equation}\label{eqtng13}
D_2 = C_1\exp \left( \frac{y_3}{L_2}+\frac{y_3}{L_1}\right) + C_2\exp \left( \frac{y_3}{L_1}-\frac{y_3}{L_2}\right)
\end{equation}
\begin{equation}
\label{eqtn:eq022}
C_1 = C_2\exp \left( \frac{-2y_3}{L_2}\right)\left( \frac{\frac{L_1}{L_2}-1}{\frac{L_1}{L_2}+1}\right)
\end{equation}
Using equations \ref{eqtng9} to \ref{eqtng12} we get;
\begin{equation}
C_2 = \Gamma(2B_2\exp \left( \frac{-y_2}{L_1}+\frac{y_2}{L_2}\right) + g_0\exp \left( \frac{y_2}{L_2}\right)
\end{equation}
were;
$\Gamma = \frac{\frac{L_1}{L_2}+ 1}{\left(\frac{L_1}{L_2}+1\right)^2 - \left(\frac{L_1}{L_2}-1\right)^2{\exp \left(\frac{-2y_3}{L_2} +\frac{2y_2}{L_2} \right)}}$








\